autoclrs/ch22-elementary-graph/main.c
@@ -4,7 +4,10 @@
 
 int main(void) {
   printf("Ch22 ImplTest: running BFS, DFS, TopologicalSort tests...\n");
-  CLRS_Ch22_ImplTestMain_run_all_tests();
+  if (!CLRS_Ch22_ImplTestMain_run_all_tests()) {
+    fprintf(stderr, "Ch22 ImplTest: FAIL\n");
+    return 1;
+  }
   printf("Ch22 ImplTest: all tests passed.\n");
   return 0;
 }
