autoclrs/ch22-elementary-graph/CLRS.Ch22.DFS.ImplTest.fsti
@@ -4,5 +4,5 @@ open Pulse.Lib.Pervasives
 
 fn test_dfs_3 ()
   requires emp
-  returns _: unit
-  ensures emp
+  returns r: bool
+  ensures emp ** pure (r == true)
